src/Safety.thy
@@ -2,33 +2,6 @@ theory Safety
   imports Main "./Raft"
 begin
 
-lemma hd_0th: "length xs > 0 \<Longrightarrow> hd xs = xs ! 0"
-  by (simp add: hd_conv_nth)
-
-definition (in raft) valid_params where
-  "valid_params n i \<equiv> (n < length all_states \<and> i < number_of_nodes)"
-
-lemma (in raft) valid_params_length_previous: "valid_params (n + 1) i \<Longrightarrow> valid_params n i"
-  by (meson add_lessD1 valid_params_def)
-
-lemma (in raft) transition_previous: "n > 0 \<Longrightarrow> (all_states ! (n - 1), all_messages ! (n - 1)) \<rightarrow> (all_states ! n, all_messages ! n)"
-  by (simp add: transition)
-
-lemma state_length_invariant_for_transition: "transition (\<sigma>, m) (\<sigma>', m') \<Longrightarrow> length \<sigma> = length \<sigma>'"
-  apply (cases rule: transition.cases)
-  apply simp+
-  done
-
-lemma (in raft) state_length_invariant: "valid_params n 0 \<Longrightarrow> length (all_states ! n) = number_of_nodes"
-  apply (induct n)
-  apply (metis hd_0th initial_state raft.valid_params_def raft_axioms repeat_length)
-  apply (metis Suc_eq_plus1 state_length_invariant_for_transition transition valid_params_length_previous)
-  done
-
-lemma leader_promote_inversion_for_transition:
-  "\<lbrakk> i < length \<sigma>; transition (\<sigma>, ms) (\<sigma>', ms'); state (\<sigma> ! i) \<noteq> leader; state (\<sigma>' ! i) = leader \<rbrakk> \<Longrightarrow> majority (length \<sigma>) (card {s. \<exists>m \<in> ms. m = message s (node i) (request_vote_response True) (currentTerm (\<sigma> ! i))})"
-  apply (cases rule: transition.cases)
-
 lemma (in raft) majority_vote_for_leader:
   "\<lbrakk> valid_params n i; state (all_states ! n ! i) = leader \<rbrakk>
   \<Longrightarrow> majority number_of_nodes (card {s. \<exists>m \<in> all_messages ! (n - 1). m = message s (node i) (request_vote_response True) (currentTerm (all_states ! (n - 1) ! i))})"
